remove dependence that Transitive-Closure requires collection framework (switch to use HOL-Library.RBT directly)

thys/Transitive-Closure/RBT_Map_Set_Extension.thy
@@ -9,11 +9,10 @@ section \<open>Accessing Values via Keys\<close>
 
 theory RBT_Map_Set_Extension
 imports
-  Collections.RBTMapImpl 
-  Collections.RBTSetImpl
+  "HOL-Library.RBT"
   Matrix.Utility
 begin
-
+ 
 text \<open>
   We provide two extensions of the red black tree implementation.
 
@@ -29,66 +28,62 @@ text \<open>
 
 subsection \<open>Subset and Union\<close>
 
-text \<open>
-  For the subset operation @{term "r \<subseteq> s"} we provide two implementations. The first one (@{term
-  rs_subset}) traverses over @{term r} and then performs membership tests \<open>\<in> s\<close>. Its
-  complexity is ${\cal O}(|r| \cdot log (|s|))$. The second one (@{term rs_subset_list}) generates
-  sorted lists for both @{term r} and @{term s} and then linearly checks the subset condition. Its
-  complexity is ${\cal O}(|r| + |s|)$.
-\<close>
+text \<open>For the subset operation @{term "r \<subseteq> s"} we provide an implementation
+  that generates
+  sorted lists for both @{term r} and @{term s} and then linearly checks the subset condition.\<close>
 
 text \<open>
   As union operator we use the standard fold function. Note that the order of the union is important
   so that new sets are added to the big union.
 \<close>
 
-(* perhaps there is a smarter way to use two iterates at the same time, however,
-  when writing this theory this feature was not detected in the RBTSetImpl theory *)
-definition rs_subset :: "('a :: linorder) rs \<Rightarrow> 'a rs \<Rightarrow> 'a option"
+definition RBT_is_key where "RBT_is_key a t = (RBT.lookup t a \<noteq> None)" 
+definition RBT_from_list where "RBT_from_list as = RBT.bulkload (map (\<lambda> x. (x,())) as)" 
+definition RBT_list_union where "RBT_list_union as bs = RBT.union bs (RBT_from_list as)" 
+definition RBT_keys where "RBT_keys t = dom (RBT.lookup t)" 
+
+lemma set_RBT_keys: "set (RBT.keys t) = RBT_keys t" 
+  unfolding RBT_keys_def by (simp add: lookup_keys)
+
+lemma RBT_from_list[simp]: "RBT_keys (RBT_from_list xs) = set xs" 
+  "set (RBT.keys (RBT_from_list xs)) = set xs" 
+proof -
+  have "x \<in> set xs \<Longrightarrow> map_of (map (\<lambda>x. (x, ())) xs) x = Some ()" for x
+    by (induct xs, auto)
+  thus "RBT_keys (RBT_from_list xs) = set xs" unfolding lookup_union lookup_bulkload RBT_from_list_def RBT_keys_def
+    by (auto dest: map_of_SomeD)
+  thus "set (RBT.keys (RBT_from_list xs)) = set xs" by (simp add: set_RBT_keys)
+qed
+
+lemmas RBT_defs = RBT_is_key_def RBT_list_union_def RBT_keys_def
+
+definition rs_subset :: "('a :: linorder,unit) RBT.rbt \<Rightarrow> ('a,unit) RBT.rbt \<Rightarrow> 'a option"
 where
-  "rs_subset as bs = rs.iteratei
-    as
-    (\<lambda> maybe. case maybe of None \<Rightarrow> True | Some _ \<Rightarrow> False)
-    (\<lambda> a _. if rs.memb a bs then None else Some a)
-    None"
+  "rs_subset as bs = sorted_list_subset (RBT.keys as) (RBT.keys bs)"
 
 lemma rs_subset [simp]:
-  "rs_subset as bs = None \<longleftrightarrow> rs.\<alpha> as \<subseteq> rs.\<alpha> bs"
-proof -
-  let ?abort = "\<lambda> maybe. case maybe of None \<Rightarrow> True | Some _ \<Rightarrow> False"
-  let ?I = "\<lambda> aas maybe. maybe = None \<longleftrightarrow> (\<forall> a. a \<in> rs.\<alpha> as - aas \<longrightarrow> a \<in> rs.\<alpha> bs)"
-  let ?it = "rs_subset as bs"
-  have "?I {} ?it \<or> (\<exists> it \<subseteq> rs.\<alpha> as. it \<noteq> {} \<and> \<not> ?abort ?it \<and> ?I it ?it)"
-    unfolding rs_subset_def
-    by (rule rs.iteratei_rule_P [where I="?I"]) (auto simp: rs.correct)
-  then show ?thesis by auto
-qed
-    
-definition rs_subset_list :: "('a :: linorder) rs \<Rightarrow> 'a rs \<Rightarrow> 'a option"
+  "rs_subset as bs = None \<longleftrightarrow> RBT_keys as \<subseteq> RBT_keys bs"
+  unfolding rs_subset_def
+  apply (subst sorted_list_subset[OF RBT.sorted_keys RBT.sorted_keys]) 
+  apply (unfold RBT_keys_def lookup_keys[symmetric])
+  by auto
+  
+definition rs_Union :: "('q :: linorder, unit) RBT.rbt list \<Rightarrow> ('q,unit) RBT.rbt"
 where
-  "rs_subset_list as bs = sorted_list_subset (rs.to_sorted_list as) (rs.to_sorted_list bs)"
-
-lemma rs_subset_list [simp]:
-  "rs_subset_list as bs = None \<longleftrightarrow> rs.\<alpha> as \<subseteq> rs.\<alpha> bs"
-  unfolding rs_subset_list_def
-    sorted_list_subset[OF rs.to_sorted_list_correct(3)[OF rs.invar, of as]
-    rs.to_sorted_list_correct(3)[OF rs.invar, of bs]]
-  by (simp add: rs.to_sorted_list_correct)
-
-definition rs_Union :: "('q :: linorder) rs list \<Rightarrow> 'q rs"
-where
-  "rs_Union = foldl rs.union (rs.empty ())"
+  "rs_Union = foldl RBT.union (RBT.empty)"
 
 lemma rs_Union [simp]:
-  "rs.\<alpha> (rs_Union qs) = \<Union> (rs.\<alpha> ` set qs)"
+  "RBT_keys (rs_Union qs) = \<Union> (RBT_keys ` set qs)"
 proof -
   { 
     fix start
-    have "rs.\<alpha> (foldl rs.union start qs) = rs.\<alpha> start \<union> \<Union> (rs.\<alpha> ` set qs)"
-      by (induct qs arbitrary: start, auto simp: rs.correct)
-  } from this[of "rs.empty ()"]
+    have "RBT_keys (foldl RBT.union start qs) = RBT_keys start \<union> \<Union> (RBT_keys ` set qs)"
+      unfolding RBT_keys_def
+      by (induct qs arbitrary: start, auto simp: RBT.lookup_union)
+  } from this[of "RBT.empty"]
   show ?thesis unfolding rs_Union_def
-    by (auto simp: rs.correct)
+    unfolding RBT_keys_def
+    by auto
 qed
 
 subsection \<open>Grouping Values via Keys\<close>
@@ -98,32 +93,22 @@ text \<open>
   rm_set_lookup}) are straight-forward, however it requires some tedious reasoning that they perform
   as they should.
 \<close>
-fun elem_list_to_rm :: "('d \<Rightarrow> 'k :: linorder) \<Rightarrow> 'd list \<Rightarrow> ('k, 'd list) rm"
+fun elem_list_to_rm :: "('d \<Rightarrow> 'k :: linorder) \<Rightarrow> 'd list \<Rightarrow> ('k, 'd list) RBT.rbt "
 where
-  "elem_list_to_rm key [] = rm.empty ()" |
+  "elem_list_to_rm key [] = RBT.empty" |
   "elem_list_to_rm key (d # ds) =
     (let
-      rm = elem_list_to_rm key ds;
+      t = elem_list_to_rm key ds;
       k = key d
     in
-      (case rm.\<alpha> rm k of
-        None \<Rightarrow> rm.update_dj k [d] rm
-      | Some data \<Rightarrow> rm.update k (d # data) rm))"
+      (case RBT.lookup t k of
+        None \<Rightarrow> RBT.insert k [d] t
+      | Some data \<Rightarrow> RBT.insert k (d # data) t))"
 
-definition "rm_set_lookup rm = (\<lambda> a. (case rm.\<alpha> rm a of None \<Rightarrow> [] | Some rules \<Rightarrow> rules))"
-
-lemma rm_to_list_empty [simp]:
-  "rm.to_list (rm.empty ()) = []" 
-proof -
-  have "map_of (rm.to_list (rm.empty ())) = Map.empty" 
-    by (simp add: rm.correct)
-  moreover have map_of_empty_iff: "\<And>l. map_of l = Map.empty \<longleftrightarrow> l = []"
-    by (case_tac l) auto
-  ultimately show ?thesis by metis
-qed
+definition "rm_set_lookup rm = (\<lambda> a. (case RBT.lookup rm a of None \<Rightarrow> [] | Some rules \<Rightarrow> rules))"
 
 locale rm_set = 
-  fixes rm :: "('k :: linorder, 'd list) rm"
+  fixes rm :: "('k :: linorder, 'd list) RBT.rbt"
     and key :: "'d \<Rightarrow> 'k"
     and data :: "'d set"
   assumes rm_set_lookup: "\<And> k. set (rm_set_lookup rm k) = {d \<in> data. key d = k}"
@@ -155,20 +140,20 @@ lemma finite_data:
 proof
   show "finite {set (rm_set_lookup rm k) | k. True}" (is "finite ?L")
   proof - 
-    let ?rmset = "rm.\<alpha> rm"
+    let ?rmset = "RBT.lookup rm"
     let ?M = "?rmset ` Map.dom ?rmset"
     let ?N = "((\<lambda> e. set (case e of None \<Rightarrow> [] | Some ds \<Rightarrow> ds)) ` ?M)"
     let ?K = "?N \<union> {{}}"
-    from rm.finite[of rm] have fin: "finite ?K" by auto 
+    have fin: "finite ?K" by auto 
     show ?thesis 
     proof (rule finite_subset[OF _ fin], rule)
       fix ds
       assume "ds \<in> ?L"
       from this[unfolded rm_set_lookup_def]
-      obtain fn where ds: "ds = set (case rm.\<alpha> rm fn of None \<Rightarrow> []
+      obtain fn where ds: "ds = set (case RBT.lookup rm fn of None \<Rightarrow> []
           | Some ds \<Rightarrow> ds)" by auto
       show "ds \<in> ?K" 
-      proof (cases "rm.\<alpha> rm fn")
+      proof (cases "RBT.lookup rm fn")
         case None
         then show ?thesis unfolding ds by auto
       next
@@ -192,7 +177,7 @@ proof
   proof (induct ds arbitrary: k)
     case Nil
     then show ?case unfolding rm_set_lookup_def 
-      by (simp add: rm.correct)
+      by simp
   next
     case (Cons d ds k)
     let ?el = "elem_list_to_rm key"
@@ -201,18 +186,18 @@ proof
     from Cons have ind:
       "\<And> k. ?l k ds = ?r k ds" by auto
     show "?l k (d # ds) = ?r k (d # ds)"
-    proof (cases "rm.\<alpha> (?el ds) (key d)")
+    proof (cases "RBT.lookup (?el ds) (key d)")
       case None
       from None ind[of "key d"] have r: "{da \<in> set ds. key da = key d} = {}"
         unfolding rm_set_lookup_def by auto
-      from None have el: "?el (d # ds) = rm.update_dj (key d) [d] (?el ds)"
+      from None have el: "?el (d # ds) = RBT.insert (key d) [d] (?el ds)"
         by simp
-      from None have ndom: "key d \<notin> Map.dom (rm.\<alpha> (?el ds))" by auto
+      from None have ndom: "key d \<notin> Map.dom (RBT.lookup (?el ds))" by auto
       have r: "?r k (d # ds) = ?r k ds \<inter> {da. key da \<noteq> key d} \<union> {da . key da = k \<and> da = d}" (is "_ = ?r1 \<union> ?r2") using r by auto
       from ndom have l: "?l k (d # ds) = 
-        set (case ((rm.\<alpha> (elem_list_to_rm key ds))(key d \<mapsto> [d])) k of None \<Rightarrow> []
+        set (case ((RBT.lookup (elem_list_to_rm key ds))(key d \<mapsto> [d])) k of None \<Rightarrow> []
         | Some rules \<Rightarrow> rules)" (is "_ = ?l") unfolding el rm_set_lookup_def 
-        by (simp add: rm.correct)
+        by simp
       {
         fix da
         assume "da \<in> ?r1 \<union> ?r2"
@@ -224,9 +209,10 @@ proof
         next
           assume "da \<in> ?r1"
           from this[unfolded ind[symmetric] rm_set_lookup_def]
-          obtain das where rm: "rm.\<alpha> (?el ds) k = Some das" and da: "da \<in> set das" and k: "key da \<noteq> key d" by (cases "rm.\<alpha> (?el ds) k", auto)
+          obtain das where rm: "RBT.lookup (?el ds) k = Some das" and da: "da \<in> set das" and k: "key da \<noteq> key d" 
+            by (cases "RBT.lookup (?el ds) k", auto)
           from ind[of k, unfolded rm_set_lookup_def] rm da k have k: "key d \<noteq> k" by auto
-          have rm: "((rm.\<alpha> (elem_list_to_rm key ds))(key d \<mapsto> [d])) k = Some das"
+          have rm: "((RBT.lookup (elem_list_to_rm key ds))(key d \<mapsto> [d])) k = Some das"
             unfolding rm[symmetric] using k by auto
           show ?thesis unfolding rm using da by auto
         qed
@@ -235,7 +221,7 @@ proof
       {
         fix da
         assume l: "da \<in> ?l"
-        let ?rm = "((rm.\<alpha> (elem_list_to_rm key ds))(key d \<mapsto> [d])) k"
+        let ?rm = "((RBT.lookup (elem_list_to_rm key ds))(key d \<mapsto> [d])) k"
         from l obtain das where rm: "?rm = Some das" and da: "da \<in> set das"
           by (cases ?rm, auto)
         have "da \<in> ?r1 \<union> ?r2" 
@@ -245,7 +231,7 @@ proof
           then show ?thesis using True by auto
         next
           case False
-          with rm have "rm.\<alpha> (?el ds) k = Some das" by auto
+          with rm have "RBT.lookup (?el ds) k = Some das" by auto
           from ind[of k, unfolded rm_set_lookup_def this] da False
           show ?thesis by auto
         qed
@@ -256,13 +242,13 @@ proof
       case (Some das)
       from Some ind[of "key d"] have das: "{da \<in> set ds. key da = key d} = set das"
         unfolding rm_set_lookup_def by auto
-      from Some have el: "?el (d # ds) = rm.update (key d) (d # das) (?el ds)"
+      from Some have el: "?el (d # ds) = RBT.insert (key d) (d # das) (?el ds)"
         by simp
-      from Some have dom: "key d \<in> Map.dom (rm.\<alpha> (?el ds))" by auto
+      from Some have dom: "key d \<in> Map.dom (RBT.lookup (?el ds))" by auto
       from dom have l: "?l k (d # ds) = 
-        set (case ((rm.\<alpha> (elem_list_to_rm key ds))(key d \<mapsto> (d # das))) k of None \<Rightarrow> []
+        set (case ((RBT.lookup (elem_list_to_rm key ds))(key d \<mapsto> (d # das))) k of None \<Rightarrow> []
         | Some rules \<Rightarrow> rules)" (is "_ = ?l") unfolding el rm_set_lookup_def 
-        by (simp add: rm.correct)
+        by simp
       have r: "?r k (d # ds) = ?r k ds \<union> {da. key da = k \<and> da = d}" (is "_ = ?r1 \<union> ?r2")  by auto
       {
         fix da
@@ -275,7 +261,7 @@ proof
         next
           assume "da \<in> ?r1"
           from this[unfolded ind[symmetric] rm_set_lookup_def]
-          obtain das' where rm: "rm.\<alpha> (?el ds) k = Some das'" and da: "da \<in> set das'" by (cases "rm.\<alpha> (?el ds) k", auto)
+          obtain das' where rm: "RBT.lookup (?el ds) k = Some das'" and da: "da \<in> set das'" by (cases "RBT.lookup (?el ds) k", auto)
           from ind[of k, unfolded rm_set_lookup_def rm] have das': "set das' = {d \<in> set ds. key d = k}" by auto
           show ?thesis 
           proof (cases "k = key d")
@@ -291,7 +277,7 @@ proof
       {
         fix da
         assume l: "da \<in> ?l"
-        let ?rm = "((rm.\<alpha> (elem_list_to_rm key ds))(key d \<mapsto> d # das)) k"
+        let ?rm = "((RBT.lookup (elem_list_to_rm key ds))(key d \<mapsto> d # das)) k"
         from l obtain das' where rm: "?rm = Some das'" and da: "da \<in> set das'"
           by (cases ?rm, auto)
         have "da \<in> ?r1 \<union> ?r2" 
@@ -310,7 +296,7 @@ proof
           from da k show ?thesis using das by auto
         next
           case False
-          with rm have "rm.\<alpha> (?el ds) k = Some das'" by auto
+          with rm have "RBT.lookup (?el ds) k = Some das'" by auto
           from ind[of k, unfolded rm_set_lookup_def this] da False
           show ?thesis by auto
         qed
